refactored

Simple_Firewall/SimpleFwSyntax.thy
@@ -1,5 +1,5 @@
 theory SimpleFwSyntax                                                                                                             
-imports Main "../Bitmagic/IPv4Addr" "../Bitmagic/BitrangeLists" "../Output_Format/Negation_Type" "../Firewall_Common_Decision_State" String
+imports Main "../Bitmagic/IPv4Addr" "../Bitmagic/BitrangeLists" "../Output_Format/Negation_Type" "../Firewall_Common_Decision_State" "../Primitive_Matchers/Iface"
 begin
 
 
@@ -18,7 +18,6 @@ section{*Simple Packet*}
 section{*Simple Firewall Syntax (IPv4)*}
   datatype protocol = ProtoAny | Proto "primitive_protocol negation_type"
 
-  datatype iface = Iface "string negation_type" | IfaceAny
   
   datatype simple_action = Accept | Drop
   
@@ -35,59 +34,6 @@ section{*Simple Firewall Syntax (IPv4)*}
   datatype simple_rule = SimpleRule simple_match simple_action
 
 section{*Simple Firewall Semantics*}
-  text{*If the interface name ends in a "+", then any interface which begins with this name will match. (man iptables)*}
-  fun cmp_iface_name :: "string \<Rightarrow> string \<Rightarrow> bool" where
-    "cmp_iface_name [] [] \<longleftrightarrow> True" |
-    "cmp_iface_name [i1] [] \<longleftrightarrow> (i1 = CHR ''+'')" |
-    "cmp_iface_name [] [i2] \<longleftrightarrow> (i2 = CHR ''+'')" |
-    "cmp_iface_name [i1] [i2] \<longleftrightarrow> (i1 = CHR ''+'' \<or> i2 = CHR ''+'' \<or> i1 = i2)" |
-    "cmp_iface_name [i1] i2s \<longleftrightarrow> (i1 = CHR ''+'')" |
-    "cmp_iface_name i1s [i2] \<longleftrightarrow> (i2 = CHR ''+'')" |
-    "cmp_iface_name (i1#i1s) (i2#i2s) \<longleftrightarrow> (if i1 = i2 then cmp_iface_name i1s i2s else False)" |
-    "cmp_iface_name _ _ \<longleftrightarrow> False"
-
-  lemma cmp_iface_name_refl: "cmp_iface_name is is"
-  proof -
-  { fix i1 i2
-    have "i1 = i2 \<Longrightarrow> cmp_iface_name i1 i2"
-      by(induction i1 i2 rule: cmp_iface_name.induct)(auto)
-   } thus ?thesis by simp 
-  qed
-  lemma cmp_iface_name_sym: "cmp_iface_name i1 i2 \<Longrightarrow> cmp_iface_name i2 i1"
-    by(induction i1 i2 rule: cmp_iface_name.induct)(auto split: split_if_asm)
-
-  lemma "cmp_iface_name (i2 # i2s) [] \<Longrightarrow> i2 = CHR ''+''"
-  proof -
-  assume a: "cmp_iface_name (i2 # i2s) []"
-  { fix x1 x2
-    have "x1 = (i2 # i2s) \<Longrightarrow> x2 = [] \<Longrightarrow> cmp_iface_name x1 x2 \<Longrightarrow> i2 = CHR ''+''"
-    by(induction x1 x2 rule: cmp_iface_name.induct) (auto)
-  } thus ?thesis using a by simp
-  qed
-  
-  text{*Examples*}
-    lemma cmp_iface_name_not_trans: "\<lbrakk>i1 = ''eth0''; i2 = ''eth+''; i3 = ''eth1''\<rbrakk> \<Longrightarrow> cmp_iface_name i1 i2 \<Longrightarrow> cmp_iface_name i2 i3 \<Longrightarrow> \<not> cmp_iface_name i1 i3"
-      by(simp)
-    lemma "cmp_iface_name ''+'' i2"
-      by(induction "''+''" i2 rule: cmp_iface_name.induct) (simp_all)
-    lemma "cmp_iface_name ''eth+'' ''eth3''" by eval
-    lemma "cmp_iface_name ''eth+'' ''e+''" by eval
-    lemma "cmp_iface_name ''eth+'' ''eth_tun_foobar''" by eval
-    lemma "cmp_iface_name ''eth+'' ''eth_tun+++''" by eval
-    lemma "\<not> cmp_iface_name ''eth+'' ''wlan+''" by eval
-    lemma "cmp_iface_name ''eth1'' ''eth1''" by eval
-    lemma "\<not> cmp_iface_name ''eth1'' ''eth2''" by eval
-    text{*If the interfaces don't end in a wildcard, then @{const cmp_iface_name} is just simple equality*}
-    lemma "\<lbrakk> hd (rev i1) \<noteq> CHR ''+''; hd (rev i2) \<noteq> CHR ''+'' \<rbrakk> \<Longrightarrow> cmp_iface_name i1 i2 \<longleftrightarrow> i1 = i2"
-      apply(induction i1 i2 rule: cmp_iface_name.induct)
-      apply(simp_all)
-      apply (metis append_Nil hd_append2 list.sel(1))+
-      done
-      
-  fun simple_match_iface :: "iface \<Rightarrow> string \<Rightarrow> bool" where
-    "simple_match_iface IfaceAny p_iface \<longleftrightarrow> True" |
-    "simple_match_iface (Iface (Pos i)) p_iface \<longleftrightarrow> cmp_iface_name p_iface i" |
-    "simple_match_iface (Iface (Neg i)) p_iface \<longleftrightarrow> \<not> cmp_iface_name p_iface i"
 
   fun simple_match_ip :: "(ipv4addr \<times> nat) negation_type \<Rightarrow> ipv4addr \<Rightarrow> bool" where
     "simple_match_ip (Pos (ip, n)) p_ip \<longleftrightarrow> p_ip \<in> ipv4range_set_from_bitmask ip n" |
@@ -104,8 +50,8 @@ section{*Simple Firewall Semantics*}
 
   fun simple_matches :: "simple_match \<Rightarrow> simple_packet \<Rightarrow> bool" where
     "simple_matches m p \<longleftrightarrow>
-      (simple_match_iface (iiface m) (p_iiface p)) \<and>
-      (simple_match_iface (oiface m) (p_oiface p)) \<and>
+      (match_iface (iiface m) (p_iiface p)) \<and>
+      (match_iface (oiface m) (p_oiface p)) \<and>
       (simple_match_ip (src m) (p_src p)) \<and>
       (simple_match_ip (dst m) (p_dst p)) \<and>
       (simple_match_proto (proto m) (p_proto p)) \<and>
